backend/CminorSel.v
@@ -141,7 +141,7 @@ Inductive state `{memory_model_ops: Mem.MemoryModelOps}: Type :=
       forall (f: fundef)                (**r fundef to invoke *)
              (args: list val)           (**r arguments provided by caller *)
              (k: cont)                  (**r what to do next  *)
-             (m: mem) (sz: Z) (tc: bool),                  (**r memory state *)
+             (m: mem) (sz: Z),                  (**r memory state *)
       state
   | Returnstate:
       forall (v: val)                   (**r return value *)
@@ -202,7 +202,7 @@ Inductive eval_expr: letenv -> expr -> val -> Prop :=
       Genv.find_funct_ptr ge b = Some (External ef) ->
       ef_sig ef = sg ->
       eval_exprlist le al vl ->
-      external_call ef ge vl m E0 v m ->
+      external_call ef ge vl (Mem.push_new_stage m) E0 v (Mem.push_new_stage m) ->
       eval_expr le (Eexternal id sg al) v
 
 with eval_exprlist: letenv -> exprlist -> list val -> Prop :=
@@ -367,7 +367,7 @@ Inductive step: state -> trace -> state -> Prop :=
       Genv.find_funct ge vf = Some fd ->
       funsig fd = sig ->
       step (State f (Scall optid sig a bl) k sp e m)
-        E0 (Callstate fd vargs (Kcall optid f sp e k) m (fn_stack_requirements id) false)
+        E0 (Callstate fd vargs (Kcall optid f sp e k) (Mem.push_new_stage m) (fn_stack_requirements id))
 
   | step_tailcall: forall f sig a bl k sp e m vf vargs fd m' id (IFI: is_function_ident ge vf id),
       eval_expr_or_symbol (Vptr sp Ptrofs.zero) e m nil a vf ->
@@ -376,7 +376,7 @@ Inductive step: state -> trace -> state -> Prop :=
       funsig fd = sig ->
       Mem.free m sp 0 f.(fn_stackspace) = Some m' ->
       step (State f (Stailcall sig a bl) k (Vptr sp Ptrofs.zero) e m)
-        E0 (Callstate fd vargs (call_cont k) m' (fn_stack_requirements id) true)
+        E0 (Callstate fd vargs (call_cont k) m' (fn_stack_requirements id))
 
   | step_builtin: forall f res ef al k sp e m vl t v m',
       list_forall2 (eval_builtin_arg sp e m) al vl ->
@@ -438,16 +438,17 @@ Inductive step: state -> trace -> state -> Prop :=
       step (State f (Sgoto lbl) k sp e m)
         E0 (State f s' k' sp e m)
 
-  | step_internal_function: forall f vargs k m m' sp e m'' sz (tc:bool),
+  | step_internal_function: forall f vargs k m m' sp e m'' sz,
       Mem.alloc m 0 f.(fn_stackspace) = (m', sp) ->
-      Mem.record_stack_blocks (if tc then m' else Mem.push_new_stage m') (make_singleton_frame_adt sp (fn_stackspace f) sz) = Some m'' ->
+      Mem.record_stack_blocks m' (make_singleton_frame_adt sp (fn_stackspace f) sz) = Some m'' ->
       set_locals f.(fn_vars) (set_params vargs f.(fn_params)) = e ->
-      step (Callstate (Internal f) vargs k m sz tc)
+      step (Callstate (Internal f) vargs k m sz)
         E0 (State f f.(fn_body) k (Vptr sp Ptrofs.zero) e m'')
-  | step_external_function: forall ef vargs k m t vres m' sz,
+  | step_external_function: forall ef vargs k m t vres m' m'' sz,
       external_call ef ge vargs m t vres m' ->
-      step (Callstate (External ef) vargs k m sz false)
-         t (Returnstate vres k m')
+      Mem.unrecord_stack_block m' = Some m'' ->
+      step (Callstate (External ef) vargs k m sz)
+         t (Returnstate vres k m'')
 
   | step_return: forall v optid f sp e k m,
       step (Returnstate v (Kcall optid f sp e k) m)
@@ -464,7 +465,7 @@ Inductive initial_state (p: program): state -> Prop :=
       funsig f = signature_main ->
       Mem.alloc m0 0 0 = (m1,b1) ->
       Mem.record_stack_blocks (Mem.push_new_stage m1) (make_singleton_frame_adt b1 0 0) = Some m2 ->
-      initial_state p (Callstate f nil Kstop m2 (fn_stack_requirements (prog_main p)) false).
+      initial_state p (Callstate f nil Kstop (Mem.push_new_stage m2) (fn_stack_requirements (prog_main p))).
 
 Inductive final_state: state -> int -> Prop :=
   | final_state_intro: forall r m,
@@ -605,9 +606,9 @@ Fixpoint funs_of_cont k : list (option (block * Z)) :=
   | stack_inv_regular: forall k f s sp m o e
                          (MSA1: match_stack_adt (Some (sp, fn_stackspace f)::funs_of_cont k) (Mem.stack_adt m)),
       stack_inv (State f s k (Vptr sp o) e m)
-  | stack_inv_call: forall k fd args m sz (tc: bool)
-                      (MSA1: match_stack_adt (funs_of_cont k) (if tc then tl (Mem.stack_adt m) else Mem.stack_adt m)),
-      stack_inv (Callstate fd args k m sz tc)
+  | stack_inv_call: forall k fd args m sz
+                      (MSA1: match_stack_adt (funs_of_cont k) (tl (Mem.stack_adt m))),
+      stack_inv (Callstate fd args k m sz)
   | stack_inv_return: forall k res m 
                         (MSA1: match_stack_adt (funs_of_cont k) (Mem.stack_adt m)),
       stack_inv (Returnstate res k m).
@@ -643,12 +644,8 @@ Fixpoint funs_of_cont k : list (option (block * Z)) :=
     - erewrite find_label_funs_of_cont by eauto.
       rewrite funs_of_call_cont.  auto.
     - apply Mem.alloc_stack_blocks in H. clear H0.
-      destruct tc.
-      + rewrite <- H, EQ1 in *. simpl in *.
-        econstructor; eauto; reflexivity.
-      + rewrite Mem.push_new_stage_stack in EQ1; inv EQ1.
-        rewrite <- H in *.
-        econstructor; eauto; reflexivity.
+      rewrite <- H, EQ1 in *. simpl in *.
+      econstructor; eauto; reflexivity.
     - simpl in MSA1. repeat destr_in MSA1. econstructor. rewrite <- H. econstructor; eauto.
   Qed.
 
