backend/LTL.v
@@ -137,7 +137,7 @@ Inductive state `{memory_model_ops: Mem.MemoryModelOps} : Type :=
       forall (stack: list stackframe) (**r call stack *)
              (f: fundef)              (**r function to call *)
              (ls: locset)             (**r location state of caller *)
-             (m: mem) (sz: Z) (tc: bool),                (**r memory state *)
+             (m: mem) (sz: Z),                (**r memory state *)
       state
   | Returnstate:
       forall (stack: list stackframe) (**r call stack *)
@@ -231,14 +231,14 @@ Inductive step: state -> trace -> state -> Prop :=
       find_function ros rs = Some fd ->
       funsig fd = sig ->
       step (Block s f sp (Lcall sig ros :: bb) rs m)
-        E0 (Callstate (Stackframe f sp rs bb :: s) fd rs m (fn_stack_requirements id) false)
+        E0 (Callstate (Stackframe f sp rs bb :: s) fd rs (Mem.push_new_stage m) (fn_stack_requirements id))
   | exec_Ltailcall: forall s f sp sig ros bb rs m fd rs' m' id (IFI: ros_is_function ros rs' id),
       rs' = return_regs (parent_locset s) rs ->
       find_function ros rs' = Some fd ->
       funsig fd = sig ->
       Mem.free m sp 0 f.(fn_stacksize) = Some m' ->
       step (Block s f (Vptr sp Ptrofs.zero) (Ltailcall sig ros :: bb) rs m)
-        E0 (Callstate s fd rs' m' (fn_stack_requirements id) true)
+        E0 (Callstate s fd rs' m' (fn_stack_requirements id))
   | exec_Lbuiltin: forall s f sp ef args res bb rs m vargs t vres rs' m',
       eval_builtin_args ge rs sp m args vargs ->
       external_call ef ge vargs m t vres m' ->
@@ -266,18 +266,19 @@ Inductive step: state -> trace -> state -> Prop :=
       Mem.unrecord_stack_block m' = Some m'' ->
       step (Block s f (Vptr sp Ptrofs.zero) (Lreturn :: bb) rs m)
         E0 (Returnstate s (return_regs (parent_locset s) rs) m'')
-  | exec_function_internal: forall s f rs m m' m'' sp rs' sz (tail: bool),
+  | exec_function_internal: forall s f rs m m' m'' sp rs' sz,
       Mem.alloc m 0 f.(fn_stacksize) = (m', sp) ->
-      Mem.record_stack_blocks (if tail then m' else Mem.push_new_stage m') (make_singleton_frame_adt sp (fn_stacksize f) sz) = Some m'' ->
+      Mem.record_stack_blocks m' (make_singleton_frame_adt sp (fn_stacksize f) sz) = Some m'' ->
       rs' = undef_regs destroyed_at_function_entry (call_regs rs) ->
-      step (Callstate s (Internal f) rs m sz tail)
+      step (Callstate s (Internal f) rs m sz)
         E0 (State s f (Vptr sp Ptrofs.zero) f.(fn_entrypoint) rs' m'')
-  | exec_function_external: forall s ef t args res rs m rs' m' sz,
+  | exec_function_external: forall s ef t args res rs m rs' m' m'' sz,
       args = map (fun p => Locmap.getpair p rs) (loc_arguments (ef_sig ef)) ->
       external_call ef ge args m t res m' ->
+      Mem.unrecord_stack_block m' = Some m'' ->
       rs' = Locmap.setpair (loc_result (ef_sig ef)) res (undef_regs destroyed_at_call rs) ->
-      step (Callstate s (External ef) rs m sz false)
-         t (Returnstate s rs' m')
+      step (Callstate s (External ef) rs m sz)
+         t (Returnstate s rs' m'')
   | exec_return: forall f sp rs1 bb s rs m,
       step (Returnstate (Stackframe f sp rs1 bb :: s) rs m)
         E0 (Block s f sp bb rs m).
@@ -298,7 +299,7 @@ Inductive initial_state (p: program): state -> Prop :=
       funsig f = signature_main ->
       Mem.alloc m0 0 0 = (m1,b1) ->
       Mem.record_stack_blocks (Mem.push_new_stage m1) (make_singleton_frame_adt b1 0 0) = Some m2 ->
-      initial_state p (Callstate nil f (Locmap.init Vundef) m2 (fn_stack_requirements (prog_main p)) false).
+      initial_state p (Callstate nil f (Locmap.init Vundef) (Mem.push_new_stage m2) (fn_stack_requirements (prog_main p))).
 
 Inductive final_state: state -> int -> Prop :=
   | final_state_intro: forall rs m retcode,
@@ -344,9 +345,9 @@ Section STACKINV.
   | stack_inv_block: forall s f sp pc rs m o
                        (MSA1: match_stack_adt (Some (sp, fn_stacksize f)::map block_of_stackframe s) (Mem.stack_adt m)),
       stack_inv (Block s f (Vptr sp o) pc rs m)
-  | stack_inv_call: forall s fd args m sz (tc: bool)
-                      (MSA1: match_stack_adt (map block_of_stackframe s) (if tc then tl (Mem.stack_adt m) else Mem.stack_adt m)),
-      stack_inv (Callstate s fd args m sz tc)
+  | stack_inv_call: forall s fd args m sz
+                      (MSA1: match_stack_adt (map block_of_stackframe s) (tl (Mem.stack_adt m))),
+      stack_inv (Callstate s fd args m sz)
   | stack_inv_return: forall s res m 
                         (MSA1: match_stack_adt (map block_of_stackframe s) (Mem.stack_adt m)),
       stack_inv (Returnstate s res m).
@@ -364,9 +365,8 @@ Section STACKINV.
     destruct 1; simpl; intros SI;
       inv SI; try econstructor; repeat rewrite_stack_blocks; eauto;
         try solve [inv MSA1; eauto].
-    - destruct tail; revert EQ1; repeat rewrite_stack_blocks; intro EQ1.
-      + rewrite EQ1 in MSA1; simpl in MSA1. econstructor; eauto; reflexivity.
-      + inv EQ1. econstructor; eauto; reflexivity.
+    - revert EQ1; repeat rewrite_stack_blocks; intro EQ1.
+      rewrite EQ1 in MSA1; simpl in MSA1. econstructor; eauto; reflexivity.
     - inv MSA1. repeat destr_in H0. econstructor. rewrite <- H. econstructor; eauto.
   Qed.
 
